Hashes and genProof left to instantiate

Extraction/src/node.ml
@@ -1,0 +1,17 @@
+open Forests
+open Protocol
+
+module Addr = Address.Addr
+module ConsensusParams = Impl.ProofOfWork
+module ForestImpl = Forests (ConsensusParams)
+module ProtocolImpl = Protocol (ConsensusParams) (ForestImpl) (Addr)
+
+let state = ref (ProtocolImpl.coq_Init 0);;
+
+let main () =
+  let argv = Array.to_list Sys.argv in
+  let args = List.tl argv in
+  Printf.printf "You are node %s\n" (string_of_int (!state).id)
+
+let () = main ()
+
